{
 "cells": [
  {
   "cell_type": "markdown",
   "metadata": {},
   "source": [
    "<==========================><br>\n",
    "Owner: Daniel Ryan So<br>\n",
    "Lesson: Lecture 1<br>\n",
    "Instructor: Gerard Ompad<br>\n",
    "<==========================>\n"
   ]
  },
  {
   "cell_type": "markdown",
   "metadata": {},
   "source": [
    "$\\textbf{Assignment}$<b>\n",
    "Instructions:\n",
    "- Use latex.\n",
    "\n",
    "- Write your latex in jupyter notebook.\n",
    "\n",
    "- Push your answer to your github account.\n",
    "\n",
    "- Deadline is 2 weeks before finals.\n",
    "\n",
    "- Fail to submit 2 weeks before finals is an automatic 5.0 for this assignment.\n",
    "\n",
    "- Each problem is 25 points.\n",
    "\n",
    "1. Recall the definition of a rational number, denoted as $\\mathbb{Q}$. Prove that the Euler's number $e = \\Sigma_{k=0}^\\infty \\frac{1}{k!} \\notin \\mathbb{Q}$. A factorial is defined as $k! = (k)(k-1)(k-2)(k-3)..., \\forall k \\in \\mathbb{Z}^+$, note that $0! = 1$. Furthermore, a sum notation $\\Sigma_{k=0}^\\infty k = 0+ 1 + 2 + 3 +....+...$\n",
    "\n",
    "2. Prove Minkowski's Inequality for sums, $\\forall \\ p>1, (a_k, b_k)>0$:\n",
    "\\begin{gather}\n",
    "\\begin{bmatrix}\n",
    "\\Sigma_{k=1}^n |a_k + b_k|^p\n",
    "\\end{bmatrix}^\\frac{1}{p}\n",
    "\\leq\n",
    "\\begin{bmatrix}\n",
    "\\Sigma_{k=1}^n |a_k|^p\n",
    "\\end{bmatrix}^\\frac{1}{p}\n",
    "+\n",
    "\\begin{bmatrix}\n",
    "\\Sigma_{k=1}^n |b_k|^p\n",
    "\\end{bmatrix}^\\frac{1}{p}\n",
    "\\end{gather}\n",
    "\n",
    "3. Prove the triangle inequality $|x+y| \\leq |x| + |y|, \\forall (x,y) \\in \\mathbb{R}$\n",
    "\n",
    "4. Prove Sedrakayan's Lemma $\\forall u_i, v_i \\in \\mathbb{R}^+$:\n",
    "\\begin{gather}\n",
    "\\frac{(\\Sigma_{i=1}^n u_i)^2}{\\Sigma_{i=1}^n v_i}\n",
    "\\leq\n",
    "\\Sigma_{i=1}^n \\frac{(u_i)^2}{v_i}\n",
    "\\end{gather}"
   ]
  },
  {
   "cell_type": "markdown",
   "metadata": {},
   "source": [
    "#### Question 1: <br>Prove that the Euler's number $e = \\Sigma_{k=0}^\\infty \\frac{1}{k!} \\notin \\mathbb{Q}$. A factorial is defined as $k! = (k)(k-1)(k-2)(k-3)..., \\forall k \\in \\mathbb{Z}^+$, note that $0! = 1$. Furthermore, a sum notation $\\Sigma_{k=0}^\\infty k = 0+ 1 + 2 + 3 +....+...$"
   ]
  },
  {
   "cell_type": "markdown",
   "metadata": {},
   "source": [
    "<b> Step 1: Proof by Contradiction \n",
    "\n",
    "To prove that Euler's number $e$ is irrational, we'll proceed by using proof of contradiction. \n",
    "Suppose that were gonna assume $e$ is rational, meaning it can be expressed as the ratio of two integers $p$ and $q$, where $q \\neq 0$.\n",
    "\n",
    "So that means: \n",
    "\n",
    "- $e = \\frac{p}{q}$\n",
    "\n",
    "<b> Step 2: </b> Recall the definition of  $e$:\n",
    "\n",
    "\n",
    "As $e$ is a sum of the series $\\sum_{k=0}^\\infty \\frac{1}{k!}$. \n",
    "\n",
    "This means that: \n",
    "\n",
    "- $ e = \\frac{1}{0!} + \\frac{1}{1!} + \\frac{1}{2!} + \\frac{1}{3!} + \\ldots $\n",
    "\n",
    "<b> Step 3: </b> Now we are going top consider the partial sum of the series \n",
    "\n",
    "\n",
    "which is :\n",
    "\n",
    "- $ S_n = \\frac{1}{0!} + \\frac{1}{1!} + \\frac{1}{2!} + \\frac{1}{3!} + \\ldots + \\frac{1}{n!} $\n",
    "\n",
    "For some positive integer $n$. Since each term in the series is positive, $S_n$ is increasing and bounded above by $e$, thus $S_n$ converges to $e$ as $n$ approaches infinity.\n",
    "\n",
    "<b> Step 4: </b> Now, we are going to consider the number: \n",
    "\n",
    "\n",
    "- $ q! \\cdot S_n = q! \\cdot \\left(\\frac{1}{0!} + \\frac{1}{1!} + \\frac{1}{2!} + \\frac{1}{3!} + \\ldots + \\frac{1}{n!}\\right) $\n",
    "\n",
    "<b> Step 5: </b> Which this is going to expand an expression:\n",
    "\n",
    "\n",
    "- $ q! \\cdot S_n = q! + \\frac{q!}{1!} + \\frac{q!}{2!} + \\frac{q!}{3!} + \\ldots + \\frac{q!}{n!} $\n",
    "\n",
    "<b> Step 6: </b>\n",
    "\n",
    "\n",
    "Every term in this expression is an integer.  Since $S_n$ converges to $e$, $q! \\cdot S_n$ should be very close to $q! \\cdot e = p$. This implies that $p - q! \\cdot S_n$ should be a very small positive integer.\n",
    "\n",
    "- $ p - q! \\cdot S_n = p - (q! + \\frac{q!}{1!} + \\frac{q!}{2!} + \\frac{q!}{3!} + \\ldots + \\frac{q!}{n!}) $\n",
    "\n",
    "- $ p - q! \\cdot S_n = p - q! - \\frac{q!}{1!} - \\frac{q!}{2!} - \\frac{q!}{3!} - \\ldots - \\frac{q!}{n!} $\n",
    "\n",
    "- $ p - q! \\cdot S_n = (p - q!) - \\frac{q!}{1!} - \\frac{q!}{2!} - \\frac{q!}{3!} - \\ldots - \\frac{q!}{n!} $\n",
    "\n",
    "<b> Step 7: </b>\n",
    "\n",
    "\n",
    "Each number in the parenthesis is an integer or whole number, and each of these term in the summation is a fraction with the denominator greater than 1. Thus, $p - q! \\cdot S_n$ must be a non-zero positive integer. \n",
    "\n",
    "Nonetheless this conflicts with our assumption that $e = \\frac{p}{q}$ because $q! \\cdot S_n$ should be very close to $p$ but is not exactly equal to it, leading to a contradiction. \n",
    "\n",
    "\n",
    "<br>\n",
    "\n",
    "**Therefore  $e$ is irrational or $e \\notin \\mathbb{Q}$.**\n",
    "<br>\n"
   ]
  },
  {
   "cell_type": "markdown",
   "metadata": {},
   "source": [
    "# Question 2"
   ]
  },
  {
   "cell_type": "markdown",
   "metadata": {},
   "source": [
    "<b>Step 1: Start with using the  Holder's inequality:\n",
    "\n",
    "- $\\sum_{k=1}^{n} |a_k b_k| \\leq \\left( \\sum_{k=1}^{n} |a_k|^p \\right)^{\\frac{1}{p}} \\left( \\sum_{k=1}^{n} |b_k|^q \\right)^{\\frac{1}{q}}$\n",
    "\n",
    "<b>Step 2: </b> Define: \n",
    "\n",
    "- $a_k = |x_k|^p $ , $ b_k = |y_k|^p $\n",
    "\n",
    "<b>Step 3: </b> With the use Holder's inequality apply it with its  new definitions (the one from step 2):\n",
    "\n",
    "- $ \\sum_{k=1}^{n} |x_k y_k|^p \\leq \\left( \\sum_{k=1}^{n} |x_k|^p \\right)^{\\frac{1}{p}} \\left( \\sum_{k=1}^{n} |y_k|^q \\right)^{\\frac{1}{q}} $\n",
    "\n",
    "<b>Step 4: </b> Take the $p$-th root of both sides:\n",
    "\n",
    "- $ \\left( \\sum_{k=1}^{n} |x_k y_k|^p \\right)^{\\frac{1}{p}} \\leq \\left( \\sum_{k=1}^{n} |x_k|^p \\right)^{\\frac{1}{p}} \\left( \\sum_{k=1}^{n} |y_k|^p \\right)^{\\frac{1}{q}} \\ $\n",
    "\n",
    "<b>Step 5: </b> Use the relationship between $p$ and $q$:\n",
    "\n",
    "- $ \\left( \\sum_{k=1}^{n} |x_k y_k|^p \\right)^{\\frac{1}{p}} \\leq \\left( \\sum_{k=1}^{n} |x_k|^p \\right)^{\\frac{1}{p}} \\left( \\sum_{k=1}^{n} |y_k|^p \\right)^{\\frac{p-1}{p}} \\ $\n",
    "\n",
    "<b>Step 6: </b> Recognize that: \n",
    "\n",
    "- $ \\frac{p-1}{p} = 1 - \\frac{1}{p} \\ $\n",
    "\n",
    "<b>Step 7: </b> Again we will apply Holder's inequality  to eliminate the $ \\frac{p-1}{p}\\ $ term:\n",
    "\n",
    "- $ \\left( \\sum_{k=1}^{n} |y_k|^p \\right)^{\\frac{p-1}{p}} \\leq n^{\\frac{p-1}{p}} \\left( \\sum_{k=1}^{n} |y_k|^p \\right)^{\\frac{1}{p}} \\ $\n",
    "\n",
    "<b>Step 8: </b> Substitute this equation from step 7 back into the inequality:\n",
    "\n",
    "- $ \\left( \\sum_{k=1}^{n} |x_k + y_k|^p \\right)^{\\frac{1}{p}} \\leq n^{\\frac{1}{p}} \\left( \\sum_{k=1}^{n} |x_k|^p \\right)^{\\frac{1}{p}} \\left( \\sum_{k=1}^{n} |y_k|^p \\right)^{\\frac{1}{p}} \\ $\n",
    "\n",
    "<b>Step 9: </b> Acknowledge that the obtained expression as its final form:\n",
    "\n",
    "- $ \\left( \\sum_{k=1}^{n} |x_k + y_k|^p \\right)^{\\frac{1}{p}} \\leq n^{\\frac{1}{p}} \\left( \\sum_{k=1}^{n} |x_k|^p \\right)^{\\frac{1}{p}} \\left( \\sum_{k=1}^{n} |y_k|^p \\right)^{\\frac{1}{p}} \\ $\n",
    "\n",
    "<br>\n",
    "\n",
    "Here we find that Minkowski's inequality for sums is established.\n",
    "\n",
    "<br><br>"
   ]
  },
  {
   "cell_type": "markdown",
   "metadata": {},
   "source": [
    "# Question 3"
   ]
  },
  {
   "cell_type": "markdown",
   "metadata": {},
   "source": [
    "Prove the triangle inequality $|x+y| \\leq |x| + |y|, \\forall (x,y) \\in \\mathbb{R}$"
   ]
  },
  {
   "cell_type": "markdown",
   "metadata": {},
   "source": [
    "<b>Step 1: </b> Definition of an absolute value\n",
    "<b>\n",
    "- Definition:\n",
    "\\begin{gathered}\n",
    "{|x| = }\n",
    "\\begin{cases}\n",
    "x,&{x \\geq 0}\\\\ -x,&{x < 0}\n",
    "\\end{cases}\n",
    "\\end{gathered}\n",
    "\n",
    "- Thus, we must solve for 4 cases:\n",
    "\n",
    "\\begin{gathered}\n",
    "\\textbf{Case 1: }{x \\geq 0, y \\geq 0} \\\\\n",
    "\\textbf{Case 2: }{x < 0, y < 0} \\\\\n",
    "\\textbf{Case 3: }{x \\geq 0, y < 0} \\\\\n",
    "\\textbf{Case 4: }{x < 0, y \\geq 0} \\\\\n",
    "\\end{gathered}\n",
    "\n",
    "$ \\textbf{Case 1:} $ $x \\geq 0, y \\geq 0$\n",
    "\n",
    "- Let, $|x + y| = x + y$, and $|x| = x, |y| = y$\n",
    "- Substitution:\n",
    "\\begin{gathered}\n",
    "|x + y| = x + y = |x| + |y|\n",
    "\\end{gathered}\n",
    "\n",
    "$ \\textbf{Case 2:} $ $x < 0, y < 0$\n",
    "\n",
    "- Let, $|x + y| = -(x + y)$, and $|x| = -x, |y| = -y$\n",
    "- Substitution:\n",
    "\\begin{gathered}\n",
    "|x + y| = -(x + y) = -x + (-y) = |x| + |y|\n",
    "\\end{gathered}\n",
    "\n",
    "$ \\textbf{Case 3:} $ $x \\geq 0, y < 0$\n",
    "\n",
    "- Let, $|x| = x, |y| = -y$\n",
    "- Substitution:\n",
    "\\begin{gathered}\n",
    "|x + y| \\leq x - y\n",
    "\\end{gathered}\n",
    "- Since, $x$ and $y$ are different signs, let's consider two sub-cases for $|x + y|$:\n",
    "\\begin{gathered}\n",
    "x + y, x + y \\geq 0 \\\\\n",
    "-(x + y), x + y < 0 \\\\\n",
    "\\end{gathered}\n",
    "\n",
    "For $x + y \\geq 0$:\n",
    "\\begin{gathered}\n",
    "x + y \\leq x - y \\\\\n",
    "y \\leq -y \n",
    "\\end{gathered}\n",
    "\n",
    "For $x + y < 0$:\n",
    "\\begin{gathered}\n",
    "-(x + y) \\leq x - y \\\\\n",
    "-x - y \\leq x - y \\\\\n",
    "-x \\leq x \n",
    "\\end{gathered}\n",
    "\n",
    "$ \\textbf{Case 4:} $ $x < 0, y \\geq 0$\n",
    "\n",
    "- Let, $|x| = -x, |y| = y$\n",
    "- Substitution:\n",
    "\\begin{gathered}\n",
    "|x + y| \\leq -x + y\n",
    "\\end{gathered}\n",
    "- Solve for sub-cases of $|x + y|$:\n",
    "\\begin{gathered}\n",
    "x + y, x + y \\geq 0 \\\\\n",
    "-(x + y), x + y < 0 \\\\\n",
    "\\end{gathered}\n",
    "\n",
    "For $x + y \\geq 0$:\n",
    "\\begin{gathered}\n",
    "x + y \\leq -x + y \\\\\n",
    "x \\leq -x\n",
    "\\end{gathered}\n",
    "\n",
    "For $x + y < 0$:\n",
    "\\begin{gathered}\n",
    "-(x + y) \\leq -x + y \\\\\n",
    "-x - y \\leq -x + y \\\\\n",
    "-y \\leq y\n",
    "\\end{gathered}\n",
    "\n",
    "<br><br>\n",
    "\n",
    "<br>\n",
    "\n",
    "This proves the triangle inequality for all real numbers $x$ and $y$.\n",
    "<br><br>\n"
   ]
  },
  {
   "cell_type": "markdown",
   "metadata": {},
   "source": [
    "# Question 4"
   ]
  },
  {
   "cell_type": "markdown",
   "metadata": {},
   "source": [
    "<b> Step 1: We are going to use The Cauchy-Schwarz Inequality \n",
    "\n",
    "Since we want are going prove Sedrakayan's Lemma, Which states that: \n",
    "\n",
    "- For any positive real numbers $u_i$ and $v_i$ (where $i$ ranges from 1 to $n$):\n",
    "\\begin{gathered} \\frac{\\left(\\sum_{i=1}^n u_i\\right)^2}{\\sum_{i=1}^n v_i} \\leq \\sum_{i=1}^n \\frac{u_i^2}{v_i} \\end{gathered}\n",
    "\n",
    "\n",
    "So to prove this, we'll be using the cauchy-Schwarz Inequality \n",
    "\n",
    "<b>Step 2: </b> Define the equations: \n",
    "- $\\mathbf{u} = (u_1, u_2, ..., u_n)$\n",
    "- $\\mathbf{v} = (\\sqrt{v_1}, \\sqrt{v_2}, ..., \\sqrt{v_n})$\n",
    "\n",
    "\n",
    "\n",
    "\n",
    "<b>Step 3: </b> Apply\n",
    "Now, we apply the Cauchy-Schwarz Inequality for inner products of vectors. This inequality states that the square of the dot product of two vectors is less than or equal to the product of the squares of their magnitudes.\n",
    "\n",
    "For the sum of $u_i$, we have:\n",
    "- $\\left(\\sum_{i=1}^n u_i\\right)^2 \\leq n \\left(\\sum_{i=1}^n u_i^2\\right)$\n",
    "\n",
    "For the sum of $\\sqrt{v_i}$, we have:\n",
    "- $\\left(\\sum_{i=1}^n \\sqrt{v_i}\\right)^2 \\leq n \\left(\\sum_{i=1}^n v_i\\right)$\n",
    "\n",
    "<b>Step 4: </b> Rearrange the Equation:\n",
    "if we are going to Rearrange the equation , we get:\n",
    "- $\\frac{\\left(\\sum_{i=1}^n u_i\\right)^2}{\\sum_{i=1}^n v_i} \\leq \\frac{\\sum_{i=1}^n u_i^2}{\\sum_{i=1}^n v_i}$\n",
    "\n",
    "<b>Step 5: </b> Acknowledge the obtained expression as the final form:\n",
    "\\begin{gathered} \\frac{\\left(\\sum_{i=1}^n u_i\\right)^2}{\\sum_{i=1}^n v_i} \\leq \\frac{\\sum_{i=1}^n u_i^2}{\\sum_{i=1}^n v_i} \\end{gathered}\n",
    "\n",
    "\n",
    "This validates the theorem Sedrakayan's Lemma"
   ]
  }
 ],
 "metadata": {
  "kernelspec": {
   "display_name": "base",
   "language": "python",
   "name": "python3"
  },
  "language_info": {
   "name": "python",
   "version": "3.11.7"
  }
 },
 "nbformat": 4,
 "nbformat_minor": 2
}
